Attempt to prove soundness of commands

practice.v
@@ -5,8 +5,11 @@ Require Import Coq.Arith.Even.
 Require Import Parity.
 Require Import Maps.
 Require Import Language.
+Require Import Aux.
 
 Definition state := total_map nat.
+
+Definition abstract_state := total_map (parity).
 
 
 (* Find some way to define eval and abstract_eval on the same 
@@ -34,10 +37,10 @@ Fixpoint eval_bexp (st : state) (e : bexp) : bool :=
   | BAnd b1 b2 => andb (eval_bexp st b1) (eval_bexp st b2)
   end.
 
-Fixpoint abstract_eval_aexp (st : state) (e : aexp) : parity :=
+Fixpoint abstract_eval_aexp (st : abstract_state) (e : aexp) : parity :=
   match e with 
   | ANum n => extract n
-  | AVar x => extract (st x)
+  | AVar x => (st x)
   | APlus p1 p2 => 
       parity_plus (abstract_eval_aexp st p1) (abstract_eval_aexp st p2)
   | AMult p1 p2 =>
@@ -54,7 +57,7 @@ Fixpoint ceval (st : state) (c : com) : state :=
       ceval st' c2
   end.
 
-Fixpoint ceval_abstract (st : state) (c : com) : state :=
+Fixpoint ceval_abstract (st : abstract_state) (c : com) : abstract_state :=
   match c with
   | CSkip => st
   | c1 ;; c2 =>
@@ -171,44 +174,58 @@ Proof.
   - inversion H.
 Qed.
 
-Lemma abstract_aexp_plus_sound : forall st e1 e2,
-  gamma (abstract_eval_aexp st e1) (eval_aexp st e1) ->
-  gamma (abstract_eval_aexp st e2) (eval_aexp st e2) ->
-  gamma (abstract_eval_aexp st (APlus e1 e2)) (eval_aexp st (APlus e1 e2)).
+Lemma abstract_aexp_plus_sound : forall st ast e1 e2,
+  gamma (abstract_eval_aexp ast e1) (eval_aexp st e1) ->
+  gamma (abstract_eval_aexp ast e2) (eval_aexp st e2) ->
+  gamma (abstract_eval_aexp ast (APlus e1 e2)) (eval_aexp st (APlus e1 e2)).
 Proof.
   intros. simpl. apply gamma_distr_plus; assumption.
 Qed.
 
-Lemma abstract_aexp_mult_sound : forall st e1 e2,
-  gamma (abstract_eval_aexp st e1) (eval_aexp st e1) ->
-  gamma (abstract_eval_aexp st e2) (eval_aexp st e2) ->
-  gamma (abstract_eval_aexp st (AMult e1 e2)) (eval_aexp st (AMult e1 e2)).
+Lemma abstract_aexp_mult_sound : forall ast st e1 e2,
+  gamma (abstract_eval_aexp ast e1) (eval_aexp st e1) ->
+  gamma (abstract_eval_aexp ast e2) (eval_aexp st e2) ->
+  gamma (abstract_eval_aexp ast (AMult e1 e2)) (eval_aexp st (AMult e1 e2)).
 Proof. intros. simpl. apply gamma_distr_mult; assumption.
 Qed.
 
-Theorem abstract_aexp_eval_sound : forall st x n p e,
-  st x = n ->
-  extract n = p ->
-  (gamma p) n ->
-  (gamma (abstract_eval_aexp st e)) (eval_aexp st e).
+Theorem abstract_aexp_eval_sound : forall ast st e,
+  (forall x, gamma (ast x) (st x)) ->
+  (gamma (abstract_eval_aexp ast e)) (eval_aexp st e).
 Proof.
   induction e; intros.
   - (* ANum *)
     simpl. apply gamma_extract_n_n.
   - (* AVar *)
-    simpl. apply gamma_extract_n_n.
+    simpl. apply H.
   - (* APlus *)
     apply abstract_aexp_plus_sound; auto.
   - (* AMult *)
     apply abstract_aexp_mult_sound; auto.
 Qed.
 
-Theorem abstract_ceval_sound : forall st x n p c,
-  st x = n ->
-  extract n = p ->
-  (gamma p) n ->
-  (gamma ((ceval_abstract st c) x)) ((ceval st c) x).
+Theorem abstract_ceval_seq_sound : forall ast c1 c2 x st,
+  gamma ((ceval_abstract ast c1) x) ((ceval st c1) x) ->
+  gamma (ceval_abstract ast (c1;; c2) x) (ceval st (c1;; c2) x).
 Proof.
+  intros. simpl. induction c2.
+  - auto.
+  - simpl in *.
+
+Admitted.
+
+Theorem abstract_ceval_sound : forall ast st c x,
+  (forall x, gamma (ast x) (st x)) ->
+  (gamma ((ceval_abstract ast c) x)) ((ceval st c) x).
+Proof.
+  intros. induction c.
+  - (* SKIP *)
+    intros. simpl. apply H.
+  - (* CSeq *)
+    apply abstract_ceval_seq_sound.
+Qed.
+    
+
 
 (* proof the equivalance of the galois connection diagram *)
 (* Peval o gamma \subset gamma o abstract_eval *)
@@ -216,3 +233,5 @@ Proof.
 
 (* Add a statements SKIP, sequencing, if statements, assignment *)
 
+(* TODO abstract store *)
+(* TODO abstract bool *)
