Makefile
@@ -1,0 +1,24 @@
+all: practice.vo
+
+SOURCES=$(wildcard %.v)
+OBJECTS=$(patsubst %.v,%.vo,$(SOURCES))
+
+
+.PHONY: all
+
+practice.vo: Aux.vo Language.vo Maps.vo Parity.vo
+	coqc practice.v
+
+Aux.vo:
+	coqc Aux.v
+
+Language.vo:
+	coqc Language.v
+
+Maps.vo:
+	coqc Maps.v
+
+Parity.vo:
+	coqc Parity.v
+
+
